Documentation.

src/dafny/beacon/gasper/GasperFinalisation.dfy
@@ -1,5 +1,5 @@
 /*
- * Copyright 2020 ConsenSys Software Inc.
+ * Copyright 2021 ConsenSys Software Inc.
  *
  * Licensed under the Apache License, Version 2.0 (the "License"); you may 
  * not use this file except in compliance with the License. You may obtain 
@@ -71,44 +71,37 @@ module GasperFinalisation {
     }
 
     /**
-     *  
-     *  @param  i       An index in the sequence of ebbs. This is not the epoch
-     *                  of a checkpoint but rather the epoch is |ebbs| - 1 - i 
-     *  @param  xb      A sequence of block roots from most recent to genesis root.
-     *  @param  ebbs    A sequence of indices. (xb[ebbs(j)],j) is EBB(xb, |ebbs| - 1 - j).
-     *                  The last element (xb[ebbs[|ebbs| - 1]], |ebbs| - 1 - (|ebbs| - 1) )
-     *                  i.e. (xb[|xb| - 1], 0) is assumed to be justified.
-     *  @param  links   All the attestations received so far.
-     *  @returns        Whether (xb[ebbs[i]], i) is 2-finalised according to the votes in *                  `links`.         
-     *  @note           ebbs contains EBB for epochs |ebbs| - 1 down to 0. 
+     *  Two finalisation.
+     *
+     *  @param  cp      A check point.
+     *  @param  store   A store.
+     *  @returns        True iff the cp is 2-finalised in the store.
+     *
+     *  @note           This new definition has not been used in the proofs.
+     *                  It is not guaranteed that it is correct but can easily be fixed if not.
      */
-    // predicate isTwoFinalised(i: nat, xb : seq<Root>, ebbs: seq<nat>,  links : seq<PendingAttestation>)
-    //     /** i is an index in ebbs, and each index represents an epoch so must be uint64.
-    //      *  i is not the first or second index as to be 1-finalised it needs to have at least on descendant.
-    //      */
-    //     requires 1 < i < |ebbs|  <= 0x10000000000000000
-    //     // requires 0 < i 
-    //     /** `xb` has at least two blocks. */
-    //     requires |xb| >= 3
-    //     /** The last element of ebbs is the EBB at epoch 0 and should be the last block in `xb`. */
-    //     requires ebbs[|ebbs| - 1] == |xb| - 1
-        
-    //     /** (xb[ebbs[j]], j) is the EBB at epoch |ebbs| - j and must be an index in `xb`.  */
-    //     requires forall i :: 0 <= i < |ebbs| ==> ebbs[i] < |xb|
-
-    //     decreases |ebbs| - i 
-    // {
-    //     //  2-finalised
-    //     isJustified(i, xb, ebbs, links) &&
-    //     //  index i - 1 is justified two 
-    //     isJustified(i - 1, xb, ebbs, links) &&
-    //     //  index i - 2 is justified by i
-    //     //  note: the EBBs are in reverse order in `ebbs`
-    //     |collectValidatorsAttestatingForLink(
-    //         links, 
-    //         CheckPoint(i as Epoch, xb[ebbs[i]]),                //  source
-    //         CheckPoint((i - 2) as Epoch, xb[ebbs[i - 2]]))|     //  target
-    //              >= (2 * MAX_VALIDATORS_PER_COMMITTEE) / 3 + 1
-    // }
-
+    predicate isTwoFinalised(cp: CheckPoint, store: Store) 
+        /** The block root must in the store.  */
+        requires cp.root in store.blocks.Keys      
+        requires 0 <= cp.epoch as nat + 2 <= MAX_UINT64 
+   
+        /** The store is well-formed, each block with slot != 0 has a parent
+            which is itself in the store. */
+        requires isClosedUnderParent(store)
+        requires isSlotDecreasing(store)  
+    {
+        //  cp is justified
+        isJustified(cp, store)
+        //  it justifies a checkpoint at epoch cp.epoch + 2
+        && exists cp2 : CheckPoint ::
+            cp2.epoch == cp.epoch + 2
+            && cp2.root in store.blocks.Keys 
+            && cp.root in chainRoots(cp2.root, store)
+            && |collectValidatorsAttestatingForLink(store.rcvdAttestations, cp, cp2)| >= (2 * MAX_VALIDATORS_PER_COMMITTEE) / 3 + 1   
+        && exists cp1 : CheckPoint ::
+            cp1.epoch == cp.epoch + 2
+            && cp1.root in store.blocks.Keys 
+            && cp.root in chainRoots(cp1.root, store)
+            && isJustified(cp1, store)
+    }
 }
